theories/generic/utp_value.thy
@@ -7,7 +7,7 @@
 header {* Abstract Values *}
 
 theory utp_value
-imports "../utp_common" "../utp_sorts"
+imports "../utp_common" "../utp_sorts2"
 begin
 
 subsection {* Locale @{term "VALUE"} *}
@@ -39,6 +39,32 @@ theorem carrier_member [intro!] :
 "x : t \<Longrightarrow> x \<in> carrier t"
 apply (auto simp: carrier_def type_non_empty)
 done
+
+subsection {* Type Coercion *}
+
+definition coerce_type :: "'TYPE \<Rightarrow> 'VALUE \<Rightarrow> 'VALUE" where
+"coerce_type t v \<equiv> if (v : t) then v else (SOME v. v : t)"
+
+lemma coerce_type: "coerce_type t v : t"
+  apply(simp add:coerce_type_def)
+  apply(clarify)
+  apply(rule someI_ex)
+  apply(rule type_non_empty)
+done
+
+lemma coerce_value: "v : t \<Longrightarrow> coerce_type t v = v"
+  by (simp add:coerce_type_def)
+
+subsection {* Set Coercion *}
+
+definition coerce_set :: "'VALUE set \<Rightarrow> 'VALUE \<Rightarrow> 'VALUE" where
+"coerce_set s v \<equiv> if (v \<in> s) then v else (SOME v. v \<in> s)"
+
+lemma coerce_set: "\<exists>v. v \<in> s \<Longrightarrow> coerce_set s x \<in> s"
+  by (auto simp add:coerce_set_def)
+
+lemma coerce_set_type: "\<lbrakk> \<forall>x \<in> s. x : t; \<exists>x. x \<in> s \<rbrakk>  \<Longrightarrow> (coerce_set s v) : t"
+  by (auto simp add:coerce_set_def)
 
 subsection {* Value Sets *}
 
@@ -76,20 +102,47 @@ end
 
 locale BOOL_VALUE = VALUE "type_rel" 
   for     type_rel :: "'VALUE :: BOOL_SORT \<Rightarrow> 'TYPE \<Rightarrow> bool" (infix ":" 50) +  
-  fixes   BoolType :: "'TYPE"
-  assumes IsBool_type: "y : BoolType \<longleftrightarrow> IsBool y"
+  fixes   BoolType :: "'TYPE" ("\<bool>") 
+  assumes BoolSort_type: "y : \<bool> \<longleftrightarrow> y \<in> BoolSort"
 
 locale INT_VALUE  = VALUE "type_rel"
   for     type_rel :: "'VALUE :: INT_SORT \<Rightarrow> 'TYPE \<Rightarrow> bool" (infix ":" 50) + 
-  fixes   IntType :: "'TYPE"
-  assumes IsInt_type: "y : IntType \<longleftrightarrow> IsInt y"
+  fixes   IntType :: "'TYPE" ("\<int>")
+  assumes IntSort_type: "y : \<int> \<longleftrightarrow> y \<in> IntSort"
 
+(*
 locale STRING_VALUE  = VALUE "type_rel"
   for     type_rel :: "'VALUE :: STRING_SORT \<Rightarrow> 'TYPE \<Rightarrow> bool" (infix ":" 50) + 
   fixes   StringType :: "'TYPE"
   assumes IsString_type: "y : StringType \<longleftrightarrow> IsString y"
+*)
 
-locale BASIC_VALUE = BOOL_VALUE "type_rel" + INT_VALUE "type_rel" + STRING_VALUE "type_rel"
-  for type_rel :: "'VALUE :: BASIC_SORT \<Rightarrow> 'TYPE \<Rightarrow> bool" (infix ":" 50)
+locale FUNCTION_VALUE = VALUE "type_rel"
+  for     type_rel ::  "'VALUE :: FUNCTION_SORT \<Rightarrow> 'TYPE \<Rightarrow> bool" (infix ":" 50) + 
+  fixes   FuncType ::  "'TYPE \<Rightarrow> 'TYPE \<Rightarrow> 'TYPE" (infixr "=p\<Rightarrow>" 60)
+  and     in_type  ::  "'TYPE \<Rightarrow> 'TYPE"
+  and     out_type ::  "'TYPE \<Rightarrow> 'TYPE"
+  assumes WF_FUNC_type: "\<And> f a b. \<lbrakk> MkFunc f : a =p\<Rightarrow> b \<rbrakk> \<Longrightarrow> f \<in> WF_FUNC"
+  and     MkFunc_type: "f ` carrier a \<subseteq> carrier b \<Longrightarrow> MkFunc f : a =p\<Rightarrow> b"
+  and     FuncApp_type: "\<And> f. \<lbrakk> f : a =p\<Rightarrow> b; x : a \<rbrakk> \<Longrightarrow> f $ x : b"
+  and     FuncType_in[simp]:  "in_type  (a =p\<Rightarrow> b) = a"
+  and     FuncType_out[simp]: "out_type (a =p\<Rightarrow> b) = b"
+
+locale PARTIAL_FUNCTION_VALUE = VALUE "type_rel"
+  for     type_rel  :: "'VALUE :: PARTIAL_FUNCTION_SORT \<Rightarrow> 'TYPE \<Rightarrow> bool" (infix ":" 50) + 
+  fixes   PFuncType :: "'TYPE \<Rightarrow> 'TYPE \<Rightarrow> 'TYPE" (infixr "~p\<Rightarrow>" 60)
+  and     pin_type  :: "'TYPE \<Rightarrow> 'TYPE"
+  and     pout_type :: "'TYPE \<Rightarrow> 'TYPE"
+  assumes WF_PFUNC_type: "\<And> f a b. \<lbrakk> MkPFunc f : a ~p\<Rightarrow> b \<rbrakk> \<Longrightarrow> f \<in> WF_PFUNC"
+(*  and     MkPFunc_type: "ran (f |` carrier a) \<subseteq> carrier b \<Longrightarrow> MkPFunc f : a ~p\<Rightarrow> b" *)
+  and     MkPFunc_type: "\<lbrakk> dom f \<subseteq> carrier a; ran f \<subseteq> carrier b \<rbrakk>  \<Longrightarrow> MkPFunc f : a ~p\<Rightarrow> b"
+  and     AppPFunc_type: "\<And> f. \<lbrakk> f : a ~p\<Rightarrow> b; x \<in> dom (DestPFunc f)  \<rbrakk> 
+                          \<Longrightarrow> f $$ x : b"
+  and     AppPFunc_ntype: "\<And> f. \<lbrakk> f : a ~p\<Rightarrow> b;  \<not> (v : a) \<rbrakk> \<Longrightarrow> DestPFunc f v = None"
+  and     PFuncType_in[simp]:  "pin_type  (a ~p\<Rightarrow> b) = a"
+  and     PFuncType_out[simp]: "pout_type (a ~p\<Rightarrow> b) = b"
+
+locale BASIC_VALUE = FUNCTION_VALUE "type_rel" + PARTIAL_FUNCTION_VALUE "type_rel" + BOOL_VALUE "type_rel" (* + INT_VALUE "type_rel" + STRING_VALUE "type_rel" *)
+  for type_rel :: "'VALUE :: CORE_SORT \<Rightarrow> 'TYPE \<Rightarrow> bool" (infix ":" 50)
 
 end
